IMP-/IMP_To_IMP-/Binary_Operations.thy
@@ -1,4 +1,5 @@
 \<^marker>\<open>creator Florian Keßler\<close>
+\<^marker>\<open>creator Fabian Huch\<close>
 
 section "Binary Operations in IMP-"
 
@@ -81,39 +82,39 @@ lemma larvs_set_enum: "lvarS c = set (enumerate_variables c)"
 
 fun binary_assign_constant_bits:: "nat \<Rightarrow> vname \<Rightarrow> nat \<Rightarrow> IMP_Minus_com" where
 "binary_assign_constant_bits 0 v x = SKIP" |
-"binary_assign_constant_bits (Suc n) v x = (var_bit_to_var (v, n)) ::= nth_bit x n ;;
+"binary_assign_constant_bits (Suc n) v x = (var_bit_to_var (v, (Suc n))) ::= nth_bit x n ;;
   binary_assign_constant_bits n v x"
 
 lemma result_of_binary_assign_constant_bits: "t_small_step_fun (3 * n)
   (binary_assign_constant_bits n v x, s)
   = (SKIP, \<lambda>w. (case var_to_var_bit w of
-      Some (w', m) \<Rightarrow> (if w' = v \<and> m < n then Some (nth_bit x m) else s w) |
+      Some (w', Suc m) \<Rightarrow> (if w' = v \<and> m < n then Some (nth_bit x m) else s w) |
       _ \<Rightarrow> s w))"
 proof(induction n arbitrary: s)
   case (Suc n)
   thus ?case
     apply auto
     apply(rule seq_terminates_when[where ?t1.0=1 and ?t2.0="3*n" and
-          ?s3.0="s(var_bit_to_var (v, n) \<mapsto> nth_bit x n)"])
-    by(auto simp: fun_eq_iff var_to_var_bit_eq_Some_iff  split: option.splits)
-qed (auto simp: fun_eq_iff split: option.splits)
+          ?s3.0="s(var_bit_to_var (v, Suc n) \<mapsto> nth_bit x n)"])
+    by(auto simp: fun_eq_iff var_to_var_bit_eq_Some_iff  split: option.splits nat.splits)
+qed (auto simp: fun_eq_iff split: option.splits nat.splits)
 
 lemma binary_assign_constant_bits_variables[simp]: 
-  "set (enumerate_variables (binary_assign_constant_bits n v x)) = { var_bit_to_var (v, i) | i. i < n }"
+  "set (enumerate_variables (binary_assign_constant_bits n v x)) = { var_bit_to_var (v, Suc i) | i. i < n }"
   apply(induction n)
   by(auto simp: set_enumerate_variables_seq)
 
 definition binary_assign_zero :: "nat \<Rightarrow> vname \<Rightarrow> nat \<Rightarrow> IMP_Minus_com" where
-"binary_assign_zero n v x = (var_bit_to_var (v, n)) ::= zero_bit x n"
+"binary_assign_zero n v x = (var_bit_to_var (v, 0)) ::= zero_bit x n"
 
 lemma result_of_binary_assign_zero: "t_small_step_fun 1
   (binary_assign_zero n v x, s) 
   = (SKIP, \<lambda>w. (case var_to_var_bit w of
-      Some (w',m) \<Rightarrow> (if w' = v \<and> m = n then Some (zero_bit x m) else s w ) | _ \<Rightarrow> s w))"
+      Some (w',m) \<Rightarrow> (if w' = v \<and> m = 0 then Some (zero_bit x n) else s w ) | _ \<Rightarrow> s w))"
   unfolding binary_assign_zero_def
   by (auto simp: numeral_eq_Suc var_to_var_bit_eq_Some_iff fun_eq_iff split: option.splits)
 
-lemma binary_assign_zero_vars: "enumerate_variables (binary_assign_zero n v x) = [var_bit_to_var (v,n)]"
+lemma binary_assign_zero_vars: "enumerate_variables (binary_assign_zero n v x) = [var_bit_to_var (v,0)]"
   unfolding binary_assign_zero_def by simp
 
 definition "binary_assign_constant n v x = binary_assign_zero n v x;; binary_assign_constant_bits n v x"
@@ -126,17 +127,20 @@ lemma result_of_binary_assign_constant:
   "t_small_step_fun (3 * n + 2)
   (binary_assign_constant n v x, s)
   = (SKIP, \<lambda>w. (case var_to_var_bit w of
-      Some (w', m) \<Rightarrow> (if w' = v \<and> m < n then Some (nth_bit x m) else if w' = v \<and> m = n then Some (zero_bit x m) else s w) |
+      Some (w', m) \<Rightarrow> if w' = v then 
+        (case m of 0 \<Rightarrow> Some (zero_bit x n)
+                 | Suc m \<Rightarrow> if m < n then Some (nth_bit x m) else s w)
+        else s w |
       _ \<Rightarrow> s w))"
   unfolding binary_assign_constant_def
   apply (rule seq_terminates_when[of 1 "3*n"])
   apply simp
    apply (rule result_of_binary_assign_zero)
   apply (subst result_of_binary_assign_constant_bits[of n v x])
-  by (auto simp add: fun_eq_iff split: option.splits if_splits)
+  by (auto simp add: fun_eq_iff split: option.splits if_splits nat.splits)
 
 lemma binary_assign_constant_variables[simp]: "set (enumerate_variables (binary_assign_constant n v x))
-  = {var_bit_to_var (v, i) | i. i < n} \<union> { var_bit_to_var (v, n)}"
+  = {var_bit_to_var (v, Suc i) | i. i < n} \<union> { var_bit_to_var (v, 0)}"
   apply (subst larvs_set_enum[symmetric]) 
   unfolding binary_assign_constant_def binary_assign_zero_def
   apply auto
@@ -155,7 +159,7 @@ lemma result_of_binary_assign_constant_on_translated_state_aux:
   unfolding IMP_State_To_IMP_Minus_def
   using result_of_binary_assign_constant_bits[of n v x] 
   by (simp add: fun_eq_iff
-  IMP_State_To_IMP_Minus_with_operands_a_b_def split: option.splits)
+  IMP_State_To_IMP_Minus_with_operands_a_b_def split: option.splits nat.splits)
 
 lemma result_of_binary_assign_constant_on_translated_state:
   assumes "n > 0"
@@ -170,7 +174,7 @@ lemma result_of_binary_assign_constant_on_translated_state:
 fun copy_var_to_operand:: "nat \<Rightarrow> char \<Rightarrow> vname \<Rightarrow> IMP_Minus_com" where
 "copy_var_to_operand 0 op v = SKIP" |
 "copy_var_to_operand (Suc i) op v =
-   (IF var_bit_to_var (v, i) \<noteq>0 THEN
+   (IF var_bit_to_var (v, Suc i) \<noteq>0 THEN
    (operand_bit_to_var (op, i)) ::= One
     ELSE
     (operand_bit_to_var (op, i)) ::= Zero) ;;
@@ -180,7 +184,7 @@ lemma copy_var_to_operand_result:
   "t_small_step_fun (4 * n) (copy_var_to_operand n op v, s)
   = (SKIP, \<lambda>w. (case var_to_operand_bit w of
     Some (op', i) \<Rightarrow> (if op' = op \<and> i < n
-  then (case s (var_bit_to_var (v, i)) of Some x \<Rightarrow> Some x | None \<Rightarrow> Some One)
+  then (case s (var_bit_to_var (v, Suc i)) of Some x \<Rightarrow> Some x | None \<Rightarrow> Some One)
   else s w) |
     _ \<Rightarrow> s w))"
 proof(induction n arbitrary: s)
@@ -189,10 +193,10 @@ proof(induction n arbitrary: s)
 next
   case (Suc n)
   let ?s' = "s(operand_bit_to_var (op, n)
-    \<mapsto> (case s (var_bit_to_var (v, n)) of Some x \<Rightarrow> x | None \<Rightarrow> One))"
+    \<mapsto> (case s (var_bit_to_var (v, Suc n)) of Some x \<Rightarrow> x | None \<Rightarrow> One))"
   show ?case using Suc
     by(auto simp: fun_eq_iff var_to_operand_bit_eq_Some_iff numeral_3_eq_3 less_Suc_eq_le
-      split!: option.splits if_splits
+      split!: option.splits if_splits nat.splits
       intro!: seq_terminates_when[where ?t1.0=3 and ?t2.0="4 * n" and ?s3.0="?s'"])
 qed
 
@@ -228,16 +232,16 @@ definition copy_atom_to_operand:: "nat \<Rightarrow> char \<Rightarrow> AExp.ato
 lemma copy_atom_to_operand_a_result:
   "t_small_step_fun (4 * n) (copy_atom_to_operand n (a_chr) a,
    IMP_State_To_IMP_Minus_with_operands_a_b s n b c)
-  = (SKIP,  IMP_State_To_IMP_Minus_with_operands_a_b s n (AExp.atomVal a s) c)"
-  by(auto simp: copy_atom_to_operand_def fun_eq_iff copy_const_to_operand_result
+  = (SKIP, IMP_State_To_IMP_Minus_with_operands_a_b s n (AExp.atomVal a s) c)"
+  by (auto simp: copy_atom_to_operand_def fun_eq_iff copy_const_to_operand_result
       copy_var_to_operand_result IMP_State_To_IMP_Minus_with_operands_a_b_def
       var_to_operand_bit_eq_Some_iff
-      split!: option.splits AExp.atomExp.splits char.splits bool.splits)
+      split!: option.splits AExp.atomExp.splits char.splits bool.splits nat.splits)
 
 lemma copy_atom_to_operand_b_result:
   "t_small_step_fun (4 * n) (copy_atom_to_operand n (b_chr) a,
    IMP_State_To_IMP_Minus_with_operands_a_b s n b c)
-  = (SKIP,  IMP_State_To_IMP_Minus_with_operands_a_b s n b (AExp.atomVal a s))"
+  = (SKIP, IMP_State_To_IMP_Minus_with_operands_a_b s n b (AExp.atomVal a s))"
   by(auto simp: copy_atom_to_operand_def fun_eq_iff copy_const_to_operand_result
       copy_var_to_operand_result IMP_State_To_IMP_Minus_with_operands_a_b_def
       var_to_operand_bit_eq_Some_iff
@@ -246,7 +250,7 @@ lemma copy_atom_to_operand_b_result:
 lemma copy_atom_to_operand_variables:
   "set (enumerate_variables (copy_atom_to_operand n op a))
     = { operand_bit_to_var (op, i) | i. i < n }
-    \<union> { var_bit_to_var (v, i) | i v. i < n \<and> v \<in> set (vars a) }"
+    \<union> { var_bit_to_var (v, Suc i) | i v. i < n \<and> v \<in> set (vars a) }"
   apply (induction n)
   apply(cases a)
     apply (auto simp: copy_atom_to_operand_def enumerate_variables_def)[1]
@@ -258,13 +262,13 @@ lemma copy_atom_to_operand_variables:
 definition assign_var_carry::
   "nat \<Rightarrow> vname \<Rightarrow> nat \<Rightarrow> nat \<Rightarrow> nat \<Rightarrow> nat \<Rightarrow> IMP_Minus_com" where
 "assign_var_carry i v a b c z =
-  (var_bit_to_var (v, i)) ::= (if a + b + c = 1 \<or> a + b + c = 3 then One else Zero) ;;
+  (var_bit_to_var (v, Suc i)) ::= (if a + b + c = 1 \<or> a + b + c = 3 then One else Zero) ;;
   carry ::= (if a + b + c \<ge> 2 then One else Zero) ;;
   zero ::= (if z = 0 \<and> (a + b + c = 0 \<or> a + b + c = 2) then Zero else One)"
 
 lemma result_of_assign_var_carry:
   "t_small_step_fun 7 (assign_var_carry i v a b c z, s)
-    = (SKIP, s(var_bit_to_var (v, i) \<mapsto> (if a + b + c = 1 \<or> a + b + c = 3 then One else Zero),
+    = (SKIP, s(var_bit_to_var (v, Suc i) \<mapsto> (if a + b + c = 1 \<or> a + b + c = 3 then One else Zero),
      carry \<mapsto> (if a + b + c \<ge> 2 then One else Zero),
       zero \<mapsto> (if z = 0 \<and> (a + b + c = 0 \<or> a + b + c = 2) then Zero else One)))"
   by(auto simp: assign_var_carry_def t_small_step_fun_terminate_iff)
@@ -315,17 +319,15 @@ lemma full_adder_correct:
     "s (operand_bit_to_var (a_chr, i)) = Some (nth_bit a i)"
     "s (operand_bit_to_var (b_chr, i)) = Some (nth_bit b i)"
   shows "t_small_step_fun 11 (full_adder i v, s) = (SKIP,
-    s(var_bit_to_var (v, i) \<mapsto> nth_bit (a + b) i, carry \<mapsto> nth_carry i a b, zero \<mapsto> zero_bit (a + b) (i + 1)))"
+    s(var_bit_to_var (v, Suc i) \<mapsto> nth_bit (a + b) i, carry \<mapsto> nth_carry i a b, zero \<mapsto> zero_bit (a + b) (i + 1)))"
   using assms
   apply(simp add: full_adder_def Let_def t_small_step_fun_terminate_iff result_of_assign_var_carry)
   apply(cases i)
    apply (simp_all add: fun_eq_iff first_bit_of_add nth_bit_of_add zero_bit_rec)
   done
 
-
-
 lemma full_adder_variables: "set (enumerate_variables (full_adder i v)) =
-  { operand_bit_to_var (a_chr, i), operand_bit_to_var (b_chr, i), var_bit_to_var (v, i),
+  { operand_bit_to_var (a_chr, i), operand_bit_to_var (b_chr, i), var_bit_to_var (v, Suc i),
     carry, zero}"
   apply (subst larvs_set_enum[symmetric])
   unfolding full_adder_def by (auto simp: Let_def assign_var_carry_def)
@@ -339,20 +341,20 @@ lemma sequence_of_full_adders:
   shows
    "t_small_step_fun (13 * k) (com_list_to_seq (map (\<lambda>i. full_adder i v) [0..< k]), s)
   = (SKIP, (\<lambda>w. (case var_to_var_bit w of
-    Some (w', m) \<Rightarrow> (if w' = v \<and> m < k then Some (nth_bit (a + b) m) else s w) |
+    Some (w', Suc m) \<Rightarrow> (if w' = v \<and> m < k then Some (nth_bit (a + b) m) else s w) |
     _ \<Rightarrow> (if w = carry \<and> k > 0 then Some (nth_carry (k-1) a b)
           else if w = zero then Some (zero_bit (a+b) k)
           else s w))))"
   using assms
 proof(induction k)
   case 0
-  with assms(1,2) show ?case by (auto simp: fun_eq_iff split: option.splits)
+  with assms(1,2) show ?case by (auto simp: fun_eq_iff split: option.splits nat.splits)
 next
   case (Suc k)
   let ?s = 
     "(\<lambda>w. case var_to_var_bit w of
-      Some (w', m) \<Rightarrow> if w' = v \<and> m < k then Some (nth_bit (a + b) m) else s w
-    | None \<Rightarrow> 
+      Some (w', Suc m) \<Rightarrow> if w' = v \<and> m < k then Some (nth_bit (a + b) m) else s w
+    | _ \<Rightarrow> 
       if w = carry \<and> 0 < k then Some (nth_carry (k - 1) a b) else
       if w = zero then Some (zero_bit (a + b) k) 
       else s w)"
@@ -366,15 +368,15 @@ next
     by simp
   let ?s2 =
     "(\<lambda>w. case var_to_var_bit w of
-      Some (w', m) \<Rightarrow> if w' = v \<and> m < Suc k then Some (nth_bit (a + b) m) else s w
-    | None \<Rightarrow>
+      Some (w', Suc m) \<Rightarrow> if w' = v \<and> m < Suc k then Some (nth_bit (a + b) m) else s w
+    | _ \<Rightarrow>
       if w = carry \<and> 0 < Suc k then Some (nth_carry (Suc k - 1) a b) else 
       if w = zero then Some (zero_bit (a + b) (Suc k))
       else s w)"
 
   have 2: "t_small_step_fun 11 ((full_adder k v), ?s) = (SKIP, ?s2)"
     apply (subst full_adder_correct)
-    by (auto simp: Suc.prems fun_eq_iff var_to_var_bit_eq_Some_iff split!: if_splits option.splits)
+    by (auto simp: Suc.prems fun_eq_iff var_to_var_bit_eq_Some_iff split!: if_splits option.splits nat.splits)
   have "map (\<lambda>i. full_adder i v) [0..<Suc k] = (map (\<lambda>i. full_adder i v) [0..<k]) @ [full_adder k v]" by simp
   with 1 2 show ?case
     apply simp
@@ -386,36 +388,41 @@ qed
 definition write_zero where
 "write_zero n v = 
   IF zero\<noteq>0 THEN 
-    (var_bit_to_var (v, n)) ::= One
-   ELSE (var_bit_to_var (v, n)) ::= Zero;;
+    (var_bit_to_var (v, 0)) ::= One
+   ELSE (var_bit_to_var (v, 0)) ::= Zero;;
    carry ::= Zero ;;
    zero ::= Zero"
 
 lemma result_write_zero: "t_small_step_fun 6
      (write_zero n v,
       \<lambda>w. case var_to_var_bit w of
-          None \<Rightarrow>
+         Some (w', Suc m) \<Rightarrow>
+            
+            if w' = v \<and> m < n then Some (nth_bit c m)
+            else IMP_State_To_IMP_Minus_with_operands_a_b s n a b w
+       | _ \<Rightarrow>
             if w = carry \<and> 0 < n then Some cv else
             if w = zero then Some (zero_bit c n) else
-            IMP_State_To_IMP_Minus_with_operands_a_b s n a b w
-        | Some (w', m) \<Rightarrow> 
-            if w' = v \<and> m < n then Some (nth_bit c m)
-            else IMP_State_To_IMP_Minus_with_operands_a_b s n a b w) =
+            IMP_State_To_IMP_Minus_with_operands_a_b s n a b w)
+         =
     (SKIP,
      \<lambda>w. case var_to_var_bit w of
           None \<Rightarrow>
             if w = carry then Some Zero else
             if w = zero then Some Zero else
             IMP_State_To_IMP_Minus_with_operands_a_b s n a b w
-        | Some (w', m) \<Rightarrow>
-            if w' = v \<and> m = n then Some (zero_bit ((s(v := c)) w') m) else 
-            if w' = v \<and> m < n then Some (nth_bit c m)
+        | Some (w', m) \<Rightarrow> 
+            if w' = v then (
+              case m of 0 \<Rightarrow> Some (zero_bit ((s(v := c)) w') n)
+            | Suc m \<Rightarrow>
+                 if m < n then Some (nth_bit c m) else 
+                 IMP_State_To_IMP_Minus_with_operands_a_b s n a b w)
             else IMP_State_To_IMP_Minus_with_operands_a_b s n a b w)"
   unfolding write_zero_def
-  by (auto simp: numeral_eq_Suc simp: fun_eq_iff var_to_var_bit_eq_Some_iff split: if_splits option.splits)
+  by (auto simp: numeral_eq_Suc simp: fun_eq_iff var_to_var_bit_eq_Some_iff split: if_splits option.splits nat.splits)
 
 lemma write_zero_vars[simp]: 
-  "set (enumerate_variables (write_zero n v)) = {zero, carry, var_bit_to_var (v,n)}"
+  "set (enumerate_variables (write_zero n v)) = {zero, carry, var_bit_to_var (v,0)}"
   unfolding write_zero_def
   apply (subst larvs_set_enum[symmetric])
   by auto
@@ -437,7 +444,7 @@ lemma result_of_adder:
   apply (auto simp: fun_eq_iff var_to_var_bit_eq_Some_iff IMP_State_To_IMP_Minus_with_operands_a_b_def
       split!: option.splits if_splits)
   apply (subst result_write_zero)
-  apply (auto simp: IMP_State_To_IMP_Minus_with_operands_a_b_def split: if_splits option.splits)
+  apply (auto simp: IMP_State_To_IMP_Minus_with_operands_a_b_def split: if_splits option.splits nat.splits)
   done
 
 definition binary_adder:: "nat \<Rightarrow> vname \<Rightarrow> AExp.atomExp \<Rightarrow> AExp.atomExp \<Rightarrow> IMP_Minus_com" where
@@ -467,7 +474,7 @@ section \<open>Subtraction\<close>
 definition assign_var_carry_sub::
   "nat \<Rightarrow> vname \<Rightarrow> nat \<Rightarrow> nat \<Rightarrow> nat \<Rightarrow> nat \<Rightarrow> IMP_Minus_com" where
 "assign_var_carry_sub i v a b c z =
-  (var_bit_to_var (v, i)) ::= 
+  (var_bit_to_var (v, Suc i)) ::= 
     (if b + c = 0 \<or> b + c = 2 then (if a = 1 then One else Zero)
      else (if b + c = 1 \<and> a = 0 then One else Zero)) ;;
   carry ::= (if a < b + c then One else Zero);;
@@ -475,7 +482,7 @@ definition assign_var_carry_sub::
 
 lemma result_of_assign_var_carry_sub:
   "t_small_step_fun 7 (assign_var_carry_sub i v a b c z, s)
-    = (SKIP, s(var_bit_to_var (v, i) \<mapsto> (if b + c = 0 \<or> b + c = 2 then (if a = 1 then One else Zero)
+    = (SKIP, s(var_bit_to_var (v, Suc i) \<mapsto> (if b + c = 0 \<or> b + c = 2 then (if a = 1 then One else Zero)
     else (if b + c = 1 \<and> a = 0 then One else Zero)),
      carry \<mapsto>  (if a < b + c then One else Zero), 
      zero \<mapsto> (if z = 0 \<and> ((a + b + c = 0) \<or> (b + c = 2 \<and> a = 0) \<or> (b + c = 1 \<and> a = 1)) then Zero else One)))"
@@ -527,15 +534,15 @@ lemma full_subtractor_correct_no_underflow:
     "s (operand_bit_to_var (a_chr, i)) = Some (nth_bit a i)"
     "s (operand_bit_to_var (b_chr, i)) = Some (nth_bit b i)"
   shows "t_small_step_fun 11 (full_subtractor i v, s) = (SKIP,
-    s(var_bit_to_var (v, i) \<mapsto> nth_bit (a - b) i, carry \<mapsto> nth_carry_sub i a b, zero \<mapsto> zero_bit (a - b) (i + 1)))"
+    s(var_bit_to_var (v, Suc i) \<mapsto> nth_bit (a - b) i, carry \<mapsto> nth_carry_sub i a b, zero \<mapsto> zero_bit (a - b) (i + 1)))"
   using assms
-  apply(simp add: full_subtractor_def Let_def t_small_step_fun_terminate_iff result_of_assign_var_carry_sub)
+  apply(simp add: full_subtractor_def Let_def t_small_step_fun_terminate_iff result_of_assign_var_carry_sub split: nat.splits)
   apply(cases i)
-  apply (simp_all add: fun_eq_iff first_bit_of_sub_n_no_underflow nth_bit_of_sub_n_no_underflow Let_def zero_bit_rec)
+   apply (simp_all add: fun_eq_iff first_bit_of_sub_n_no_underflow nth_bit_of_sub_n_no_underflow Let_def zero_bit_rec)
   done
 
 lemma full_subtractor_variables: "set (enumerate_variables (full_subtractor i v)) =
-  { operand_bit_to_var (a_chr, i), operand_bit_to_var (b_chr, i), var_bit_to_var (v, i),
+  { operand_bit_to_var (a_chr, i), operand_bit_to_var (b_chr, i), var_bit_to_var (v, Suc i),
     carry, zero}"
   apply (subst larvs_set_enum[symmetric])
   unfolding full_subtractor_def Let_def
@@ -550,21 +557,21 @@ lemma sequence_of_full_subtractors_no_underflow:
   shows
    "t_small_step_fun (13 * n) (com_list_to_seq (map (\<lambda>i. full_subtractor i v) [0..< n]), s)
   = (SKIP, (\<lambda>w. (case var_to_var_bit w of
-    Some (w', m) \<Rightarrow> (if w' = v \<and> m < n then Some (nth_bit (a - b) m) else s w) |
+    Some (w', Suc m) \<Rightarrow> (if w' = v \<and> m < n then Some (nth_bit (a - b) m) else s w) |
     _ \<Rightarrow> (if w = carry \<and> n > 0 then Some (nth_carry_sub (n - 1) a b)
           else if w = zero then Some (zero_bit (a-b) n)
           else s w))))"
   using assms
 proof(induction n)
   case 0
-  with assms(1,2) show ?case by (auto simp: fun_eq_iff split: option.splits)
+  with assms(1,2) show ?case by (auto simp: fun_eq_iff split: option.splits nat.splits)
 next
   case (Suc n)
   have "t_small_step_fun (13 + 13 * n)
    (com_list_to_seq ((map (\<lambda>i. full_subtractor i v) [0..< n]) @ [full_subtractor n v]), s)
     = (SKIP, (\<lambda>w. (case var_to_var_bit w of
-      Some (w', m) \<Rightarrow> (if w' = v \<and> m < Suc n then Some (nth_bit (a - b) m) else s w) |
-      None \<Rightarrow> 
+      Some (w', Suc m) \<Rightarrow> (if w' = v \<and> m < Suc n then Some (nth_bit (a - b) m) else s w) |
+      _ \<Rightarrow> 
         (if w = carry \<and> Suc n > 0 then Some (nth_carry_sub n a b) else
          if w = zero then Some (zero_bit (a-b) (Suc n))
          else s w))))"
@@ -573,7 +580,8 @@ next
     using Suc  apply(auto)
     apply(subst full_subtractor_correct_no_underflow)
     using Suc
-    by(auto simp add: fun_eq_iff var_to_var_bit_eq_Some_iff split!: option.splits)
+    apply (auto simp add: fun_eq_iff var_to_var_bit_eq_Some_iff split!: option.splits nat.splits if_splits)
+    done
   thus ?case by auto
 qed
 
@@ -587,7 +595,7 @@ lemma sequence_of_full_subtractors_with_underflow:
   shows
    "t_small_step_fun (13 * n) (com_list_to_seq (map (\<lambda>i. full_subtractor i v) [0..< n]), s)
   = (SKIP, (\<lambda>w. (case var_to_var_bit w of
-    Some (w', m) \<Rightarrow> (if w' = v \<and> m < n then Some (nth_bit (2^n + a - b) m) else s w) |
+    Some (w', Suc m) \<Rightarrow> (if w' = v \<and> m < n then Some (nth_bit (2^n + a - b) m) else s w) |
     _ \<Rightarrow> (if w = carry \<and> n > 0 then Some One
           else if w = zero then Some (zero_bit (2^n + a - b) n)
           else s w))))"
@@ -599,7 +607,7 @@ proof -
   ultimately have "t_small_step_fun (13 * n)
                        (com_list_to_seq (map (\<lambda>i. full_subtractor i v) [0..< n]), s)
   = (SKIP, (\<lambda>w. (case var_to_var_bit w of
-    Some (w', m) \<Rightarrow> (if w' = v \<and> m < n then Some (nth_bit (2^n + a - b) m) else s w) |
+    Some (w', Suc m) \<Rightarrow> (if w' = v \<and> m < n then Some (nth_bit (2^n + a - b) m) else s w) |
     _ \<Rightarrow> (if w = carry \<and> n > 0 then Some (nth_carry_sub (n - 1) (2^n + a) b) else
           if w = zero then Some (zero_bit (2^n + a - b) n)
           else s w))))"
@@ -616,7 +624,7 @@ IF carry\<noteq>0 THEN
   binary_assign_constant n v 0)
 ELSE SKIP)"
 
-(* proper setup... why was this not done before ?! *)
+text \<open>Intro rules for easy reasoning:\<close>
 
 lemma seq_intro:
  "t_small_step_fun n1 (c1,s) = (SKIP,s2) \<Longrightarrow> 
@@ -655,13 +663,14 @@ lemma result_underflow_handler_carry: "s carry \<noteq> Some Zero \<Longrightarr
             else if w = zero then Some Zero
             else s w
           | Some (w', m) \<Rightarrow>
-              if w' = v \<and> m < n then Some (nth_bit 0 m)
-              else if w' = v \<and> m = n then Some (zero_bit 0 m)
+              if w' = v then case m of
+                0 \<Rightarrow> Some (zero_bit 0 n)
+              | Suc m \<Rightarrow> if m < n then Some (nth_bit 0 m) else s w
               else s w))"
   unfolding underflow_handler_def
   apply (auto  intro!:  intros ifTrue_intro)
   apply (subst t_small_step_fun_increase_time[OF _ result_of_binary_assign_constant])
-   apply (auto split!: if_splits option.splits)
+   apply (auto split!: if_splits option.splits nat.splits)
   done
 
 lemma result_underflow_handler_carry_Skip: "s carry = Some Zero \<Longrightarrow>
@@ -697,7 +706,8 @@ proof(cases "a < b")
     apply (subst result_underflow_handler_carry)
      apply (auto)
     unfolding write_zero_def
-    apply (auto  simp: numeral_eq_Suc simp: fun_eq_iff var_to_var_bit_eq_Some_iff IMP_State_To_IMP_Minus_with_operands_a_b_of_changed_s_neq_iff split: if_splits option.splits)
+    apply (auto  simp: numeral_eq_Suc simp: fun_eq_iff var_to_var_bit_eq_Some_iff 
+        IMP_State_To_IMP_Minus_with_operands_a_b_of_changed_s_neq_iff split: if_splits option.splits nat.splits)
      defer using zero_bit_one apply fastforce
     using IMP_State_To_IMP_Minus_with_operands_a_b_of_changed_s_neq_iff
     by (metis not_Some_eq)
@@ -713,7 +723,8 @@ next
      apply (subst result_underflow_handler_carry_Skip)
       apply auto
     unfolding write_zero_def
-    apply (auto simp: numeral_eq_Suc simp: fun_eq_iff var_to_var_bit_eq_Some_iff IMP_State_To_IMP_Minus_with_operands_a_b_of_changed_s_neq_iff split: if_splits option.splits)
+     apply (auto simp: numeral_eq_Suc simp: fun_eq_iff var_to_var_bit_eq_Some_iff 
+        IMP_State_To_IMP_Minus_with_operands_a_b_of_changed_s_neq_iff split: if_splits option.splits nat.splits)
     apply (metis One_nat_def assms(2,3) nth_carry_sub_no_underflow
         verit_comp_simplify1(3))
      using nth_carry_sub_no_underflow[OF _ \<open>a < 2 ^ n\<close> \<open>b < 2 ^ n\<close>]
@@ -726,11 +737,12 @@ qed
 lemma subtract_handle_underflow_variables:
   "set (enumerate_variables (subtract_handle_underflow n v))
   = { operand_bit_to_var (op, i) | i op. i < n \<and> (op = a_chr \<or> op = b_chr) }
-    \<union> { var_bit_to_var (v, i) | i. i < n }
-    \<union> { carry, zero, var_bit_to_var (v, n) }"
-  by(auto simp: subtract_handle_underflow_def
+    \<union> { var_bit_to_var (v, i) | i. i \<le> n }
+    \<union> { carry, zero }"
+  apply (auto simp: subtract_handle_underflow_def gr0_conv_Suc
        set_enumerate_variables_seq com_list_to_seq_variables full_subtractor_variables
        set_enumerate_variables_if underflow_handler_def)
+  done
 
 definition binary_subtractor:: "nat \<Rightarrow> vname \<Rightarrow> AExp.atomExp \<Rightarrow> AExp.atomExp \<Rightarrow> IMP_Minus_com" where
 "binary_subtractor n v a b =
